Pick related lemmas need constraint about well formedness of dtyp

src/coq/DynamicTypes.v
@@ -47,12 +47,95 @@ Inductive dtyp : Set :=
 | DTYPE_Struct (fields:list dtyp)
 | DTYPE_Packed_struct (fields:list dtyp)
 | DTYPE_Opaque
+                                   (* IY: Why isn't this defined structurally? *)
 | DTYPE_Vector (sz:Z) (t:dtyp)     (* t must be integer, floating point, or pointer type *)
 .
 
+Definition vector_dtyp dt :=
+  (exists n, dt = DTYPE_I n) \/ dt = DTYPE_Pointer \/ dt = DTYPE_Half \/ dt = DTYPE_Float \/
+        dt = DTYPE_Double \/ dt = DTYPE_X86_fp80 \/ dt = DTYPE_Fp128 \/ dt = DTYPE_Ppc_fp128.
+
+Section DtypInd.
+  Variable P : dtyp -> Prop.
+  Hypothesis IH_I             : forall a, P (DTYPE_I a).
+  Hypothesis IH_Pointer       : P DTYPE_Pointer.
+  Hypothesis IH_Void          : P DTYPE_Void.
+  Hypothesis IH_Half          : P DTYPE_Half.
+  Hypothesis IH_Float         : P DTYPE_Float.
+  Hypothesis IH_Double        : P DTYPE_Double.
+  Hypothesis IH_X86_fp80      : P DTYPE_X86_fp80.
+  Hypothesis IH_Fp128         : P DTYPE_Fp128.
+  Hypothesis IH_Ppc_fp128     : P DTYPE_Ppc_fp128.
+  Hypothesis IH_Metadata      : P DTYPE_Metadata.
+  Hypothesis IH_X86_mmx       : P DTYPE_X86_mmx.
+  Hypothesis IH_Array         : forall sz t, P t -> P (DTYPE_Array sz t).
+  Hypothesis IH_Struct        : forall (fields: list dtyp), (forall u, In u fields -> P u) -> P (DTYPE_Struct fields).
+  Hypothesis IH_Packed_Struct : forall (fields: list dtyp), (forall u, In u fields -> P u) -> P (DTYPE_Packed_struct fields).
+  Hypothesis IH_Opaque        : P DTYPE_Opaque.
+  Hypothesis IH_Vector        : forall sz t, P t -> P (DTYPE_Vector sz t).
+
+  Lemma dtyp_ind' : forall (dt:dtyp), P dt.
+    fix IH 1.
+    remember P as P0 in IH.
+    destruct dt; auto; subst.
+    - apply IH_Array. auto.
+    - apply IH_Struct.
+      { revert fields.
+        fix IHfields 1. intros [|u fields']. intros. inversion H.
+        intros u' [<-|Hin]. apply IH. eapply IHfields. apply Hin.
+      }
+    - apply IH_Packed_Struct.
+      { revert fields.
+        fix IHfields 1. intros [|u fields']. intros. inversion H.
+        intros u' [<-|Hin]. apply IH. eapply IHfields. apply Hin.
+      }
+    - apply IH_Vector. auto.
+  Qed.
+End DtypInd.
+
+Section WF_dtyp.
+
+  Inductive well_formed_dtyp : dtyp -> Prop :=
+  | Wf_I : forall sz, well_formed_dtyp (DTYPE_I sz)
+  | Wf_Pointer : well_formed_dtyp DTYPE_Pointer
+  | Wf_Void : well_formed_dtyp DTYPE_Void
+  | Wf_Half : well_formed_dtyp DTYPE_Half
+  | Wf_Float : well_formed_dtyp DTYPE_Float
+  | Wf_Double : well_formed_dtyp DTYPE_Double
+  | Wf_X86_fp80 : well_formed_dtyp DTYPE_X86_fp80
+  | Wf_Fp128 : well_formed_dtyp DTYPE_Fp128
+  | Wf_Ppc_fp128 : well_formed_dtyp DTYPE_Ppc_fp128
+  | Wf_Metadata : well_formed_dtyp DTYPE_Metadata
+  | Wf_X86_mmx : well_formed_dtyp DTYPE_X86_mmx
+  | Wf_Opaque : well_formed_dtyp DTYPE_Opaque
+  | Wf_Array : forall (sz : Z),
+      Z.le 0 sz ->
+      forall t, well_formed_dtyp t ->
+                well_formed_dtyp (DTYPE_Array sz t)
+  | Wf_Vector : forall (sz : Z),
+      Z.le 0 sz ->
+      forall t, vector_dtyp t ->
+                well_formed_dtyp t ->
+                well_formed_dtyp (DTYPE_Vector sz t)
+  | Wf_Struct_nil :
+      well_formed_dtyp (DTYPE_Struct nil)
+  | Wf_Struct_cons :
+      forall t, well_formed_dtyp t ->
+                forall l, well_formed_dtyp (DTYPE_Struct l) ->
+                          well_formed_dtyp (DTYPE_Struct (t :: l))
+  | Wf_Packed_struct_nil :
+      well_formed_dtyp (DTYPE_Packed_struct nil)
+  | Wf_Packed_truct_cons :
+      forall t, well_formed_dtyp t ->
+                forall l, well_formed_dtyp (DTYPE_Packed_struct l) ->
+                          well_formed_dtyp (DTYPE_Packed_struct (t :: l))
+  .
+
+End WF_dtyp.
+
 Section hiding_notation.
   Local Open Scope sexp_scope.
-
+  
   Fixpoint serialize_dtyp' (dt:dtyp): sexp :=
     match dt with
     | DTYPE_I sz     => Atom ("i" ++ to_string sz)%string
